
\begin{question}
Выберите верную формулу
\begin{answerlist}
  \item \(\sum (y_i - \bar y)(x_i - \bar x) = \sum y_i x_i + \sum \bar y  \bar x\)
  \item \(\sum (y_i - \bar y)(x_i - \bar x) = \sum y_i x_i\)
  \item \(\sum (y_i - \bar y)(x_i - \bar x) = \bar y \bar x\)
  \item \(\sum (y_i - \bar y)(x_i - \bar x) = \sum y_i (x_i - \bar x)\)
  \item \(\sum (y_i - \bar y)(x_i - \bar x) = -\sum \bar y (x_i - \bar x)\)
\end{answerlist}
\end{question}

\begin{solution}
\[\sum (x_i - \bar x)=0\]
\end{solution}

