
\begin{question}
Если гипотеза \(\beta_2 + \beta_3 = 1\) верна, то модель \(\ln Y_i = \beta_1 + \beta_2 \ln X_i + \beta_3 \ln Z_i + u_i\) совпадает с моделью
\begin{answerlist}
  \item \(\ln (Y_i/Z_i) = \beta_1 + \beta_2 \ln (X_i/Z_i) + u_i\)
  \item \(\ln (Y_i/Z_i) = \beta_1 + \beta_2 \ln (Y_i/X_i) + u_i\)
  \item \(\ln (Y_i/Z_i) = \beta_1 + \beta_2 \ln (Y_i/Z_i) + u_i\)
  \item \(\ln Y_i = \beta_1 + \beta_2 \ln (X_i/Z_i) + u_i\)
  \item \(\ln Y_i = \beta_1 + \beta_2 \ln (Z_i/Y_i) + u_i\)
\end{answerlist}
\end{question}

\begin{solution}
\begin{answerlist}
  \item Good answer :)
  \item Bad answer :(
  \item Bad answer :(
  \item Bad answer :(
  \item Bad answer :(
\end{answerlist}
\end{solution}

