
\begin{question}
Показатель \(R^2_{adj}\) можно вычислить по формуле
\begin{answerlist}
  \item \(R^2_{adj} = \frac{k-1}{n-k} - R^2 \cdot \frac{n-1}{n-k}\)
  \item \(R^2_{adj} = \frac{k-1}{n-k} + R^2 \cdot \frac{n-k}{n-1}\)
  \item \(R^2_{adj} = \frac{k-1}{n-k} + R^2 \cdot \frac{n-1}{n-k}\)
  \item \(R^2_{adj} = \frac{n-k}{k-1} + R^2 \cdot \frac{n-1}{n-k}\)
  \item \(R^2_{adj} = (-1)\cdot \frac{k-1}{n-k} + R^2 \cdot \frac{n-1}{n-k}\)
  \item \(R^2_{adj} = \frac{k}{n-k} + R^2 \cdot \frac{n-1}{n-k}\)
\end{answerlist}
\end{question}

\begin{solution}
\begin{answerlist}
  \item Bad answer :(
  \item Bad answer :(
  \item Bad answer :(
  \item Bad answer :(
  \item Good answer :)
  \item Bad answer :(
\end{answerlist}
\end{solution}

