Question
========

Выберите верную формулу

Answerlist
----------
*  $\sum (y_i - \bar y)(x_i - \bar x) = \sum y_i (x_i - \bar x)$
*  $\sum (y_i - \bar y)(x_i - \bar x) = \sum y_i x_i$
*  $\sum (y_i - \bar y)(x_i - \bar x) = -\sum \bar y (x_i - \bar x)$
*  $\sum (y_i - \bar y)(x_i - \bar x) = \bar y \bar x$
*  $\sum (y_i - \bar y)(x_i - \bar x) = \sum y_i x_i + \sum \bar y  \bar x$ 

Solution
========
$$\sum (x_i - \bar x)=0$$


Meta-information
================
exname: correct formula for sums of xi yi
extype: schoice
exsolution: 10000
exshuffle: 5
exextra[Type]: Calculation
exextra[Language]: Russian
exextra[Level]: Literacy
exsection: OLS/Coefficients formula
